GameTheory/Languages/MAID/Theorems.lean
@@ -1,6 +1,7 @@
 import GameTheory.Languages.MAID.Syntax
 import GameTheory.Languages.MAID.SOS
 import GameTheory.Languages.MAID.Compile
+import GameTheory.Languages.MAID.CompileObs
 import GameTheory.Languages.MAID.Kuhn
 
 /-!
