GameTheory/Theorems.lean
@@ -1,4 +1,5 @@
 import GameTheory.Theorems.Kuhn
+import GameTheory.Theorems.Kuhn.BehavioralToMixed
 import GameTheory.Theorems.Kuhn.CorrelatedRealization
 import GameTheory.Theorems.Minimax
 import GameTheory.Theorems.NashExistence
